theories/TM/Code/BinNumbers/PosAddTM.v
@@ -417,8 +417,7 @@ Lemma Add_onto_Realise : Add_onto ⊨ Add_onto_Rel.
 Proof.
   eapply Realise_monotone.
   { unfold Add_onto. TM_Correct.
-    - apply Add_Realise.
-    - apply MoveValue_Realise with (X := positive) (Y := positive). }
+    - apply Add_Realise. }
   {
     intros tin ([], tout) H. intros p0 p1 Hp0 Hp1 Hright.
     TMSimp. modpon H. modpon H0. auto.
