theories/TM/Code/NatTM.v
@@ -174,8 +174,6 @@ Proof.
   eapply Realise_monotone.
   {
     unfold Add_Main. TM_Correct.
-    - apply CopyValue_Realise with (X := nat).
-    - apply CopyValue_Realise with (X := nat).
     - apply Add_Loop_Realise.
   }
   {
@@ -213,7 +211,6 @@ Proof.
   {
     unfold Add. TM_Correct.
     - apply Add_Main_Realise.
-    - apply Reset_Realise with (X := nat). (* Don't forget the type here! *)
   }
   {
     intros tin ((), tout) H. intros m n sx sy so s3 HEncM HEncN HOut HRight3. TMSimp.
@@ -287,10 +284,6 @@ Proof.
   unfold Add_Main, Add_Main_steps. eapply TerminatesIn_monotone.
   {
     TM_Correct.
-    - apply CopyValue_Realise with (X := nat).
-    - apply CopyValue_Terminates with (X := nat).
-    - apply CopyValue_Realise with (X := nat).
-    - apply CopyValue_Terminates with (X := nat).
     - apply Add_Loop_Terminates.
   }
   {
@@ -324,7 +317,6 @@ Proof.
     TM_Correct.
     - apply Add_Main_Realise.
     - apply Add_Main_Terminates.
-    - apply Reset_Terminates with (X := nat).
   }
   {
     intros tin k (m&n&HEncM&HEncN&HOut&HInt&Hk).
@@ -445,7 +437,6 @@ Proof.
   {
     unfold Mult_Step. TM_Correct.
     - apply Add_Computes.
-    - apply MoveValue_Realise with (X := nat).
   }
   {
     intros tin (yout, tout) H. intros c m' n sm sn sc s3 s4 HEncM' HEncN HEncC HInt3 HInt4. TMSimp.
@@ -549,7 +540,6 @@ Proof.
   eapply Realise_monotone.
   {
     unfold Mult_Main. TM_Correct.
-    - apply CopyValue_Realise with (X := nat).
     - apply Mult_Loop_Realise.
   }
   {
@@ -589,7 +579,6 @@ Proof.
   {
     unfold Mult. TM_Correct.
     - eapply Mult_Main_Realise.
-    - eapply Reset_Realise with (X := nat).
   }
   {
     intros tin ((), tout) H. cbn. intros m n sm sn so s3 s4 s5 HEncM HEncN HOut HInt3 HInt4 HInt5. TMSimp.
@@ -629,7 +618,6 @@ Proof.
     unfold Mult_Step. TM_Correct.
     - apply Add_Computes.
     - apply Add_Terminates.
-    - apply MoveValue_Terminates with (X := nat).
   }
   {
     intros tin k. intros (m'&n&c&HEncM'&HEncN&HEncC&HInt3&HInt4&Hk).
@@ -709,8 +697,6 @@ Lemma Mult_Main_Terminates : projT1 Mult_Main ↓ Mult_Main_T.
 Proof.
   eapply TerminatesIn_monotone.
   { unfold Mult_Main. TM_Correct.
-    - apply CopyValue_Realise with (X := nat).
-    - apply CopyValue_Terminates with (X := nat).
     - apply Mult_Loop_Terminates.
   }
   {
@@ -737,7 +723,6 @@ Proof.
   { unfold Mult. TM_Correct.
     - apply Mult_Main_Realise.
     - apply Mult_Main_Terminates.
-    - apply Reset_Terminates with (X := nat).
   }
   {
     intros tin k (m&n&HEncM&HEncN&HOut&HInt&Hk). cbn in *. unfold Mult_steps in Hk.
